src/Helpers/ExtrMachinePrimitives.v
@@ -1,0 +1,30 @@
+From Coq Require Import Extraction.
+From Coq Require Import ExtrHaskellBasic.
+
+From RecoveryRefinement Require Import Helpers.MachinePrimitives.
+
+(* TODO: replace fully-qualfied names here with shorter names, and add imports
+to a fiximports.py script *)
+
+Extraction Language Haskell.
+
+Extract Inlined Constant uint64 => "Data.Word.Word64".
+Extract Inlined Constant uint32 => "Data.Word.Word32".
+Extract Inlined Constant uint16 => "Data.Word.Word16".
+Extract Inlined Constant uint8  => "Data.Word.Word8".
+
+Extract Inductive comparison => "Prelude.Ordering" ["Prelude.EQ" "Prelude.LT" "Prelude.GT"].
+
+(* TODO: for now, left toNum/fromNum as undefined, but could theoretically
+extract to fromIntegral and convert to Integer (instead of nat) *)
+Extract Constant uint64_uint => "Build_UInt undefined undefined (+) (-) compare".
+Extract Constant uint32_uint => "Build_UInt undefined undefined (+) (-) compare".
+Extract Constant uint16_uint => "Build_UInt undefined undefined (+) (-) compare".
+Extract Constant uint8_uint  => "Build_UInt undefined undefined (+) (-) compare".
+
+(* TODO: need to axiomatize conversions in order to extract them to reasonable things, rather than going through Integer *)
+
+(* extract these to a real type, but don't provide any constructor *)
+Extract Inductive ByteString => "Data.ByteString.ByteString" ["undefined"].
+
+Extract Inlined Constant Fd => "System.Posix.Types.Fd".
